src/core/TermDefs.v
@@ -5,6 +5,8 @@ Require Import Monads.
 Import MonadNotations.
 Local Open Scope monad_scope.
 Require Import IntFuncs.
+Set Bullet Behavior "Strict Subproofs".
+
 (* Variable Symbols*)
 
 Record vsymbol := {
@@ -58,13 +60,6 @@ Definition lsymbol_eqb (l1 l2: lsymbol) : bool :=
   option_eqb ty_equal l1.(ls_value) l2.(ls_value) &&
   CoqBigInt.eqb l1.(ls_constr) l2.(ls_constr) &&
   Bool.eqb l1.(ls_proj) l2.(ls_proj).
-
-(*TODO: move*)
-Lemma bool_eqb_eq (b1 b2: bool) : b1 = b2 <-> Bool.eqb b1 b2.
-Proof.
-  symmetry.
-  apply eqb_true_iff.
-Qed.
 
 Lemma lsymbol_eqb_eq (l1 l2: lsymbol) : l1 = l2 <-> lsymbol_eqb l1 l2.
 Proof.
@@ -127,3 +122,152 @@ Definition create_psymbol nm al :=
 Definition ls_ty_freevars (ls: lsymbol) : Stv.t :=
   let acc := oty_freevars Stv.empty ls.(ls_value) in
   fold_left ty_freevars ls.(ls_args) acc.
+
+(* Patterns *)
+
+(*We use the same trick as with Ty, see notes there*)
+Unset Elimination Schemes.
+Record pattern_o (A: Type) :=
+  {pat_node: A; pat_vars: Svs.t; pat_ty : ty_c}.
+
+Inductive pattern_c :=
+  | mk_pat_c : pattern_node -> Svs.t -> ty_c -> pattern_c
+with pattern_node :=
+  | Pwild
+  | Pvar : vsymbol -> pattern_node
+  | Papp: lsymbol -> list pattern_c -> pattern_node
+  | Por: pattern_c -> pattern_c -> pattern_node
+  | Pas : pattern_c -> vsymbol -> pattern_node.
+
+Set Elimination Schemes.
+Definition pattern := pattern_o pattern_node.
+
+(*Again:To ensure that extraction results in correct code, we 
+  should ONLY interact with record _c types through this interface*)
+Section ExtractInterface.
+
+Definition pat_node_of (p: pattern_c) : pattern_node :=
+  match p with
+  | mk_pat_c p _ _ => p
+  end.
+
+Definition pat_vars_of (p: pattern_c) : Svs.t :=
+  match p with
+  | mk_pat_c _ s _ => s
+  end.
+
+Definition pat_ty_of (p: pattern_c) : ty_c :=
+  match p with
+  | mk_pat_c _ _ t => t
+  end.
+
+(*Constructor*)
+Definition build_pattern_o (p: pattern_node)
+  (s: Svs.t) (t: ty_c) : pattern_o pattern_node :=
+    {| pat_node := p; pat_vars := s; pat_ty := t |}.
+
+End ExtractInterface.
+
+(*TODO: go back and use this*)
+Definition mk_Forall {A: Type} {P: A -> Prop} := 
+  fun (f: forall x, P x) =>
+    fix mk_Forall (l: list A) {struct l} : Forall P l :=
+      match l with
+      | nil => Forall_nil _
+      | x :: xs => Forall_cons _ _ _ (f x) (mk_Forall xs)
+      end.
+
+(*Induction principle and decidable equality*)
+Section PatInd.
+
+Variable (P1: pattern_c -> Prop).
+Variable (P2: pattern_node -> Prop).
+Variable (Hpat: forall p, P2 (pat_node_of p) -> P1 p).
+Variable (Hwild: P2 Pwild).
+Variable (Hvar: forall v, P2 (Pvar v)).
+Variable (Happ: forall l ps, Forall P1 ps -> P2 (Papp l ps)).
+Variable (Hor: forall p1 p2, P1 p1 -> P1 p2 -> P2 (Por p1 p2)).
+Variable (Has: forall p v, P1 p -> P2 (Pas p v)).
+
+Fixpoint pattern_c_ind (p: pattern_c) : P1 p :=
+  Hpat p (pattern_node_ind (pat_node_of p))
+with pattern_node_ind (p: pattern_node) : P2 p :=
+  match p with
+  | Pwild => Hwild
+  | Pvar v => Hvar v
+  | Papp l ps => Happ l ps (mk_Forall pattern_c_ind ps)
+  | Por p1 p2 => Hor p1 p2 (pattern_c_ind p1) (pattern_c_ind p2)
+  | Pas p v => Has p v (pattern_c_ind p)
+  end.
+
+Definition pattern_mut_ind:
+  (forall p, P1 p) /\ (forall p, P2 p) :=
+  conj (fun p => pattern_c_ind p) (fun p => pattern_node_ind p).
+
+End PatInd.
+
+(*Decidable equality*)
+Fixpoint pattern_eqb (p1 p2: pattern_c) : bool :=
+  pattern_node_eqb (pat_node_of p1) (pat_node_of p2) &&
+  Svs.equal (pat_vars_of p1) (pat_vars_of p2) &&
+  ty_equal (pat_ty_of p1) (pat_ty_of p2)
+with pattern_node_eqb (p1 p2: pattern_node) : bool :=
+  match p1, p2 with
+  | Pwild, Pwild => true
+  | Pvar v1, Pvar v2 => vs_equal v1 v2
+  | Papp l1 ps1, Papp l2 ps2 =>
+    ls_equal l1 l2 &&
+    CoqBigInt.eqb (int_length ps1) (int_length ps2) &&
+    forallb (fun x => x) (map2 pattern_eqb ps1 ps2)
+  | Por p1 p2, Por p3 p4 => pattern_eqb p1 p3 &&
+    pattern_eqb p2 p4
+  | Pas p1 v1, Pas p2 v2 => pattern_eqb p1 p2 &&
+    vs_equal v1 v2
+  | _, _ => false
+  end.
+
+Lemma pattern_eqb_rewrite p1 p2:
+  pattern_eqb p1 p2 =
+  match p1, p2 with
+  | mk_pat_c p1 s1 t1, mk_pat_c p2 s2 t2 =>
+    pattern_node_eqb p1 p2 &&
+    Svs.equal s1 s2 &&
+    ty_equal t1 t2
+  end.
+Proof.
+  destruct p1; destruct p2; reflexivity.
+Qed.
+
+Lemma pattern_eqb_eq_aux:
+  (forall p1 p2, p1 = p2 <-> pattern_eqb p1 p2) /\
+  (forall p1 p2, p1 = p2 <-> pattern_node_eqb p1 p2).
+Proof.
+  apply pattern_mut_ind.
+  - intros p IH p2.
+    rewrite pattern_eqb_rewrite.
+    destruct p as [p1 s1 t1]; destruct p2 as [p2 s2 t2].
+    rewrite !andb_true, <- IH, <- ty_eqb_eq, 
+      <- (Svs.equal_eq vsymbol_eqb_eq); simpl.
+    solve_eqb_eq.
+  - intros p2; destruct p2; simpl; solve_eqb_eq.
+  - intros v p2; destruct p2; simpl; try rewrite <- vsymbol_eqb_eq;
+    solve_eqb_eq.
+  - intros l ps Hall p2. destruct p2 as [| | l2 ps2 | |];
+    try solve[solve_eqb_eq].
+    simpl.
+    rewrite !andb_true.
+    rewrite int_length_eq,<- nat_eqb_eq, <- lsymbol_eqb_eq,
+    and_assoc, <- (forall_eqb_eq Hall).
+    solve_eqb_eq.
+  - intros p1 p2 IH1 IH2 [| | | p3 p4 |]; try solve[solve_eqb_eq];
+    simpl.
+    rewrite andb_true, <- IH1, <- IH2. solve_eqb_eq.
+  - intros p v IH [| | | | p2 v2]; try solve[solve_eqb_eq]; simpl.
+    rewrite andb_true, <- IH, <- vsymbol_eqb_eq.
+    solve_eqb_eq.
+Qed.
+
+Definition pattern_eqb_eq := proj1 pattern_eqb_eq_aux.
+Definition pattern_node_eqb_eq := proj2 pattern_eqb_eq_aux.
+
+(*No sets/maps of patterns*)
